finalize expr eval proof and separate it from stmt proof

clightlight/Clightlight2ClightMatch.v
@@ -18,22 +18,37 @@ Section MATCH.
 
   Context `{Σ: GRA.t}.
   
-  Definition Es_to_eventE {A} (ms: ModSemL.t) (mn: string) (es_itree: itree Es A) (rp: p_state) :=
-     EventsL.interp_Es (ModSemL.prog ms) (transl_all mn es_itree) rp.
+  Import List.
+
+  Local Open Scope Z.
+
+  (* global env is fixed when src program is fixed *)
+  Variable sk : Sk.t.
+  Variable tge : Genv.t Clight.fundef type.
+
+  (* composite env should be fixed when src program is fixed*)
+  Variable ce : composite_env.
+
+  (* ModSem should be fixed with src too *)
+  Variable ms : ModSemL.t.
+
 
   (* should never appear *)
   Definition dummy_blk : positive := 1%positive.
 
-  Definition map_blk (defs: list (AST.ident * AST.globdef Clight.fundef Ctypes.type)) : positive -> Values.block :=
+  Definition map_blk : positive -> Values.block :=
     fun blk =>
-      if (ge_dec (Pos.to_nat blk) (S (List.length (get_sk defs))))
-      then Pos.of_nat ((List.length defs - List.length (get_sk defs)) + (Pos.to_nat blk))
+      if (Pos.of_succ_nat (length sk) <=? blk)%positive
+      then 
+        match Zpos blk + (Z.pos_sub tge.(genv_next) (Pos.of_succ_nat (length sk))) with
+        | Zpos tblk => tblk
+        | _ => dummy_blk (* unreachable *)
+        end
       else
-        let sg := Sk.load_skenv (get_sk defs) in
-        let tg := Genv.add_globals (Genv.empty_genv _ _ (List.map fst defs)) defs  in
+        let sg := Sk.load_skenv sk in
         match sg.(SkEnv.blk2id) (pred (Pos.to_nat blk)) with
         | Some name =>
-          match Genv.find_symbol tg (ident_of_string name) with
+          match Genv.find_symbol tge (ident_of_string name) with
           | Some tblk => tblk
           | None => dummy_blk
           end
@@ -41,241 +56,73 @@ Section MATCH.
         end
   .
 
-  Definition map_val defs (v : val) : val :=
+  Definition map_val (v : val) : val :=
     match v with
-    | Vptr blk ofs => Vptr (map_blk defs blk) ofs
+    | Vptr blk ofs => Vptr (map_blk blk) ofs
     | _ => v
     end.
 
-  Definition map_memval defs (mv : memval) : memval :=
+  Definition map_memval (mv : memval) : memval :=
     match mv with
-    | Fragment v q n => Fragment (map_val defs v) q n
+    | Fragment v q n => Fragment (map_val v) q n
     | _ => mv
     end.
 
-  Variant match_le defs : temp_env -> temp_env -> Prop :=
+  Variant match_ge : Prop :=
+  | match_ge_intro
+      (WFSK: Sk.wf sk)
+      (MGE: forall id idx, SkEnv.id2blk (Sk.load_skenv sk) (string_of_ident id) = Some idx -> Genv.find_symbol tge id = Some (map_blk (Pos.of_succ_nat idx)))
+    :
+      match_ge.
+
+  Variant match_le : temp_env -> temp_env -> Prop :=
   | match_le_intro
       sle tle 
-      (ML: forall id sv, Maps.PTree.get id sle = Some sv -> Maps.PTree.get id tle = Some (map_val defs sv))
+      (ML: forall id sv, Maps.PTree.get id sle = Some sv -> Maps.PTree.get id tle = Some (map_val sv))
     :
-      match_le defs sle tle.
+      match_le sle tle.
 
-  Variant match_e defs : env -> env -> Prop :=
+  Definition map_env_entry (entry: ident * (Values.block * type)) :=
+    let '(id, (b, ty)) := entry in
+    (id, (map_blk b, ty)).
+
+  Variant match_e : env -> env -> Prop :=
   | match_e_intro
       se te 
-      (ME: forall id b ty, se ! id = Some (b, ty) <-> te ! id = Some (map_blk defs b, ty))
+      (ME: Maps.PTree.elements te = List.map map_env_entry (Maps.PTree.elements se))
     :
-      match_e defs se te.
+      match_e se te.
+  
+  Lemma env_match_some e te id b ty (ME: match_e e te) :
+    e ! id = Some (b, ty) -> te ! id = Some (map_blk b, ty).
+  Proof.
+    i. apply PTree.elements_correct in H. inv ME.
+    apply PTree.elements_complete. rewrite ME0.
+    rewrite in_map_iff. eexists; split; et. ss.
+  Qed.
 
-  Variant match_ge defs : Sk.t -> Genv.t (Ctypes.fundef function) type -> Prop :=
-  | match_ge_intro
-      sk ge
-      (PUBLIC_INCL: forall s, In s (List.map fst sk) -> In (ident_of_string s) ge.(genv_public))
-      (S2B_MATCH: forall s n, (do '(blk, _) <- find_idx (fun '(s', _) => string_dec s s') sk; Some blk) = Some n -> ge.(genv_symb) ! (ident_of_string s) = Some (map_blk defs (Pos.of_succ_nat n)))
-      (B2D_MATCH: forall s n agd, nth_error sk n = Some (s, agd) -> exists gd, ge.(genv_defs) ! (map_blk defs (Pos.of_succ_nat n)) = Some gd /\ Any.downcast agd = Some gd)
-      (NEXT_MATCH: ge.(genv_next) = map_blk defs (Pos.of_succ_nat (List.length sk)))
-    :
-      match_ge defs sk ge.
-
-  (* global env is fixed when src program is fixed *)
-  Variable sk : Sk.t.
-  (* composite env should be fixed when src program is fixed*)
-  Variable ce : composite_env.
-  (* ModSem should be fixed with src too *)
-  Variable ms : ModSemL.t.
+  Lemma env_match_none e te id (ME: match_e e te) :
+    e ! id = None -> te ! id = None.
+  Proof.
+    i. destruct (te ! id) eqn : E; et. 
+    apply PTree.elements_correct in E. inv ME. rewrite ME0 in E.
+    rewrite in_map_iff in E. des. destruct x. 
+    apply PTree.elements_complete in E0. unfold map_env_entry in *.
+    destruct p0. clarify.
+  Qed.
 
 
-  Variant match_mem defs : Memory.Mem.mem -> Memory.Mem.mem -> Prop :=
+  Variant match_mem : Memory.Mem.mem -> Memory.Mem.mem -> Prop :=
   | match_mem_intro
       m tm
-      (INITIALIZED: Pos.to_nat m.(Mem.nextblock) >= (List.length (get_sk defs)))
-      (NBLK: tm.(Mem.nextblock) = map_blk defs (m.(Mem.nextblock)))
-      (MEM_CNT: forall b ofs mv, PMap.get ofs (PMap.get b m.(Mem.mem_contents)) = mv -> PMap.get ofs (PMap.get (map_blk defs b) tm.(Mem.mem_contents)) = map_memval defs mv )
-      (MEM_PERM: forall b, PMap.get b m.(Mem.mem_access) = Maps.PMap.get (map_blk defs b) tm.(Mem.mem_access) )
+      (NBLK: tm.(Mem.nextblock) = map_blk (m.(Mem.nextblock)))
+      (MEM_CNT: forall b ofs mv, PMap.get ofs (PMap.get b m.(Mem.mem_contents)) = mv -> PMap.get ofs (PMap.get (map_blk b) tm.(Mem.mem_contents)) = map_memval mv)
+      (MEM_PERM: forall b, PMap.get b m.(Mem.mem_access) = Maps.PMap.get (map_blk b) tm.(Mem.mem_access) )
     :
-      match_mem defs m tm
-  .
+      match_mem m tm.
 
-  Definition itr_t := itree Es runtime_env.
-
-  (* clightlight state should be expressed by two constructs, stmt and cont *)
-  Definition clightlight_state := itree eventE Any.t.
-
-  Definition itree_of_code (mn: string) (retty: type) (code: statement) (e: env) (le: temp_env) 
-    : stateT p_state (itree eventE) runtime_env 
-      := Es_to_eventE ms mn (decomp_stmt sk ce retty code e le).
-
-  Definition ktree_of_cont_itree (mn: string) (cont_itr: runtime_env -> itr_t)
-    : p_state * runtime_env -> itree eventE (p_state * runtime_env) 
-      := fun '(pstate, ncr) => Es_to_eventE ms mn (cont_itr ncr) pstate.
-
-  Definition itree_of_cont_pop (itr_sreturn: itr_t) (itr_sbreak: itr_t) (itr_scontinue: itr_t) (itr_skip: itr_t) 
-  : option bool -> option val -> itr_t :=
-    fun optb optv =>
-      match optv with
-      | Some _ => itr_sreturn
-      | None =>
-        match optb with
-        | Some true => itr_sbreak
-        | Some false => itr_scontinue
-        | None => itr_skip
-        end
-      end.
-
-  Definition kstop_itree (ncr: runtime_env) : itree Es val := 
-    let '(e, le, optb, optv) := ncr in
-      '(_, _, _, optv') <- (itree_of_cont_pop 
-                              (free_list_aux (ConvC2ITree.blocks_of_env ce e);;; Ret (e, le, None, optv)) 
-                              triggerUB 
-                              triggerUB 
-                              triggerUB) optb optv;; 
-      v <- optv'?;; (match v with | Vint _ => Ret v | _ => triggerUB end).
-
-  Definition itree_stop (mn: string) := fun '(pstate, ncr) => Es_to_eventE ms mn (kstop_itree ncr) pstate.
-
-    (* below is functional version of continuation translation *)
-    (*
-  Fixpoint decomp_cont (retty: type) (k: Clight.cont) (e: env) (le: temp_env) (optb: option bool) (optv: option val) : itree eff val :=
-    match k with
-    | Kseq code k' => 
-      '(e', le', optb', optv') <- (treat_flow 
-                                    (Ret (e, le, None, optv)) 
-                                    (Ret (e, le, optb, None)) 
-                                    (Ret (e, le, optb, None)) 
-                                    (decomp_stmt retty code e le)) optb optv;;
-      decomp_cont retty k' e' le' optb' optv'
-    | Kloop1 code1 code2 k' => 
-      '(e', le', optb', optv') <- (treat_flow 
-                                    (Ret (e, le, None, optv)) 
-                                    (Ret (e, le, None, None)) 
-                                    ('(e2, le2, ov2) <- sloop_iter_body_two (decomp_stmt retty code2 e le);;
-                                     match ov2 with
-                                     | Some v2 => Ret (e2, le2, None, v2)
-                                     | None => _sloop_itree e2 le2 (decomp_stmt retty code1) (decomp_stmt retty code2)
-                                     end)
-                                    ('(e2, le2, ov2) <- sloop_iter_body_two (decomp_stmt retty code2 e le);;
-                                     match ov2 with
-                                     | Some v2 => Ret (e2, le2, None, v2)
-                                     | None => _sloop_itree e2 le2 (decomp_stmt retty code1) (decomp_stmt retty code2)
-                                     end)) optb optv;;
-      decomp_cont retty k' e' le' optb' optv'
-    | Kloop2 code1 code2 k' =>
-      '(e, le, ov2) <- (match optv with 
-                        | Some v => Ret (e, le, Some (Some v)) 
-                        | None => 
-                          match optb with 
-                          | Some true => Ret (e, le, Some None)
-                          | Some false => triggerUB
-                          | None => Ret (e, le, None)
-                          end
-                        end);;
-      '(e', le', optb', optv') <- (match ov2 with
-                                  | Some v2 => Ret (e, le, None, v2)
-                                  | None => _sloop_itree e le (decomp_stmt retty code1) (decomp_stmt retty code2)
-                                  end);;
-      decomp_cont retty k' e' le' optb' optv'
-    | Kstop => 
-      '(_, _, _, optv') <- (treat_flow 
-                            (free_list_aux (blocks_of_env ce e);;; Ret (e, le, None, optv)) 
-                            triggerUB 
-                            triggerUB 
-                            triggerUB) optb optv;;
-      v <- optv'?;; (match v with Vint _ => Ret v | _ => triggerUB end)
-    | Kcall optid f e' le' k' =>
-      '(_, _, _, optv') <- (treat_flow 
-                            (free_list_aux (blocks_of_env ce e);;; tau;; Ret (e, le, None, optv)) 
-                            triggerUB 
-                            triggerUB 
-                            (free_list_aux (blocks_of_env ce e);;; tau;; Ret (e, le, None, Some Vundef))) optb optv;;
-      v <- optv'?;; decomp_cont f.(fn_return) k' e' (set_opttemp optid v le') None None
-    | _ => triggerUB
-    end.
-     *)
-
-(* mname is just module name pops the continuation *)
-  Inductive match_cont defs : type -> mname -> (p_state * runtime_env -> itree eventE (p_state * val)) -> cont -> Prop := 
-  | match_cont_Kseq cont_itree next code cont retty mn
-      (ITR: cont_itree = ktree_of_cont_itree mn 
-                        (fun '(e, le, optb, optv) => 
-                          (itree_of_cont_pop
-                            (Ret (e, le, None, optv)) 
-                            (Ret (e, le, optb, None)) 
-                            (Ret (e, le, optb, None)) 
-                            (decomp_stmt sk ce retty code e le)) optb optv))
-      (NEXT: match_cont defs retty mn next cont)
-    :
-      match_cont defs retty mn (fun x => y <- cont_itree x;; next y) (Kseq code cont)
-  | match_cont_Kloop1 cont_itree next code1 code2 cont retty mn
-      (ITR: cont_itree = ktree_of_cont_itree mn
-                        (fun '(e, le, optb, optv) => 
-                          (itree_of_cont_pop
-                            (Ret (e, le, None, optv)) 
-                            (Ret (e, le, None, None)) 
-                            ('(e2, le2, ov2) <- sloop_iter_body_two (decomp_stmt sk ce retty code2 e le);;
-                              match ov2 with
-                              | Some v2 => Ret (e2, le2, None, v2)
-                              | None => _sloop_itree e2 le2 (decomp_stmt sk ce retty code1) (decomp_stmt sk ce retty code2)
-                              end)
-                            ('(e2, le2, ov2) <- sloop_iter_body_two (decomp_stmt sk ce retty code2 e le);;
-                              match ov2 with
-                              | Some v2 => Ret (e2, le2, None, v2)
-                              | None => _sloop_itree e2 le2 (decomp_stmt sk ce retty code1) (decomp_stmt sk ce retty code2)
-                              end)) optb optv))
-      (NEXT: match_cont defs retty mn next cont) 
-    :
-      match_cont defs retty mn (fun x => y <- cont_itree x;; next y) (Kloop1 code1 code2 cont)
-  | match_cont_Kloop2 cont_itree next code1 code2 cont retty mn
-      (ITR: cont_itree = ktree_of_cont_itree mn
-                        (fun '(e, le, optb, optv) => 
-                          '(e, le, ov2) <- 
-                            (match optv with 
-                            | Some v => Ret (e, le, Some (Some v)) 
-                            | None => match optb with 
-                                      | Some true => Ret (e, le, Some None)
-                                      | Some false => triggerUB
-                                      | None => Ret (e, le, None)
-                                      end
-                            end);;
-                          match ov2 with
-                          | Some v2 => Ret (e, le, None, v2)
-                          | None => _sloop_itree e le (decomp_stmt sk ce retty code1) (decomp_stmt sk ce retty code2)
-                          end))
-      (NEXT: match_cont defs retty mn next cont) 
-    :
-      match_cont defs retty mn (fun x => y <- cont_itree x;; next y) (Kloop2 code1 code2 cont)
-  | match_cont_Kstop cont_itree retty mn
-      (ITR: cont_itree = itree_stop mn)
-    :
-      match_cont defs retty mn cont_itree Kstop
-  | match_cont_Kcall cont_itree next optid f e' le' te' tle' cont retty mn_caller mn_callee
-      (ITR: cont_itree = ktree_of_cont_itree mn_callee
-                        (fun '(e, le, optb, optv) => 
-                          '(_, _, _, optv') <-
-                            (itree_of_cont_pop
-                              (free_list_aux (ConvC2ITree.blocks_of_env ce e);;; tau;; Ret (e, le, None, optv)) 
-                              triggerUB 
-                              triggerUB 
-                              (free_list_aux (ConvC2ITree.blocks_of_env ce e);;; tau;; Ret (e, le, None, Some Vundef))) optb optv;;
-                          v <- optv'?;; Ret (e', set_opttemp optid v le', None, None))) 
-      (CONT_ENV_MATCH: match_e defs e' te')
-      (CONT_LENV_MATCH: match_le defs le' tle')
-      (NEXT: match_cont defs f.(fn_return) mn_caller next cont) 
-    :
-      match_cont defs retty mn_callee (fun x => y <- cont_itree x;; next y) (Kcall optid f te' tle' cont).
+  (* Definition env_block_prop (e: env) : Prop :=
+    forall id b ty, e ! id = Some (b, ty) -> (Pos.of_succ_nat (List.length sk) <= b)%positive. *)
   
-
-  Variant match_states defs : itree eventE Any.t -> Clight.state -> Prop :=
-  | match_states_intro
-      tf pstate e te le tle tcode m tm tcont mn itr_code itr_cont itr
-      (ML: @match_le defs le tle)
-      (ME: @match_e defs e te)
-      (PSTATE: pstate "Mem"%string = m↑)
-      (MM: @match_mem defs m tm)
-      (MCODE: itr_code = itree_of_code mn tf.(fn_return) tcode e le pstate)
-      (MCONT: match_cont defs tf.(fn_return) mn itr_cont tcont)
-      (MENTIRE: itr = x <- itr_code;; '(_, v) <- itr_cont x;; Ret v↑)
-    :
-      match_states defs itr (State tf tcode tcont te tle tm)
-  .
 
 End MATCH.
