clightlight/ConvC2ITree.v
@@ -55,13 +55,6 @@ Section EVAL_EXPR_COMP.
   Definition divide_c (n m: Z): bool :=
     let x := m / n in
     (x * n =? m).
-  
-  Definition signedness_eq sg1 sg2 : bool :=
-    match sg1, sg2 with
-    | Signed, Signed 
-    | Unsigned, Unsigned => true
-    | _, _ => false
-    end.
 
   Definition load_bitfield_c (ty: type) 
             (sz: intsize) (sg: signedness) (pos: Z) (width: Z) 
@@ -70,16 +63,18 @@ Section EVAL_EXPR_COMP.
             && (width <=? bitsize_intsize sz) 
             && (pos + width <=? Cop.bitsize_carrier sz) in
   match ty, chk with
-  | Tint sz sg1 attr, true =>
-    if signedness_eq sg1
-        (if Coqlib.zlt width (bitsize_intsize sz) 
-        then Signed else sg) 
-    then v <- ccallU "load" (Cop.chunk_for_carrier sz, addr);;
+  | Tint i sg1 attr, true =>
+    if intsize_eq i sz then
+      if signedness_eq sg1
+          (if Coqlib.zlt width (bitsize_intsize sz) 
+          then Signed else sg) 
+      then v <- ccallU "load" (Cop.chunk_for_carrier sz, addr);;
         match v with
         | Vint c => 
           Ret (Vint (Cop.bitfield_extract sz sg pos width c))
         | _ => triggerUB
         end
+      else triggerUB
     else triggerUB
   | _, _ => triggerUB
   end.
@@ -91,11 +86,12 @@ Section EVAL_EXPR_COMP.
             && (width <=? bitsize_intsize sz) 
             && (pos + width <=? Cop.bitsize_carrier sz) in
   match ty, v, chk with
-  | Tint sz sg1 attr, Vint n, true =>
-    if signedness_eq sg1
+  | Tint i sg1 attr, Vint n, true =>
+    if intsize_eq i sz then
+      if signedness_eq sg1
         (if Coqlib.zlt width (bitsize_intsize sz) 
         then Signed else sg) 
-    then v <- ccallU "load" (Cop.chunk_for_carrier sz, addr);;
+      then v <- ccallU "load" (Cop.chunk_for_carrier sz, addr);;
         match v with
         | Vint c => 
           let stored_v := Vint (Int.bitfield_insert (Cop.first_bit sz pos width) width c n) in
@@ -103,6 +99,7 @@ Section EVAL_EXPR_COMP.
           Ret (Vint (Cop.bitfield_normalize sz sg width n))
         | _ => triggerUB
         end
+      else triggerUB
     else triggerUB
   | _, _, _ => triggerUB
   end.
@@ -170,7 +167,7 @@ Section EVAL_EXPR_COMP.
           else triggerUB
         | None =>
           match SkEnv.id2blk skenv (string_of_ident id) with
-          | Some i => Ret (Pos.of_nat (S i), (Ptrofs.zero, Full))
+          | Some i => Ret (Pos.of_succ_nat i, (Ptrofs.zero, Full))
           | None => triggerUB
           end
         end
@@ -729,8 +726,8 @@ Section EVAL_EXPR_COMP.
             then Ret (Some (Ptrofs.cmpu c ofs1 ofs2))
             else Ret None
           else
-            ret1 <- ccallU "valid_pointer" (b1, ofs1);;
-            ret2 <- ccallU "valid_pointer" (b2, ofs2);;
+            ret1 <- ccallU "valid_pointer" (b1, Ptrofs.unsigned ofs1);;
+            ret2 <- ccallU "valid_pointer" (b2, Ptrofs.unsigned ofs2);;
             if
               ret1 && ret2
             then Ret (Val.cmp_different_blocks c)
@@ -928,602 +925,5 @@ Section EVAL_EXPR_COMP.
       Ret (v1'':: vs)
     | _, _ => triggerUB
     end.
-
 End EVAL_EXPR_COMP.
-
-Definition id_list_norepet_c: list ident -> bool :=
-  fun ids => if Coqlib.list_norepet_dec (ident_eq) ids then true else false.
-
-Definition id_list_disjoint_c: list ident -> list ident -> bool :=
-  fun ids1 ids2 =>
-    if (Coqlib.list_disjoint_dec ident_eq ids1 ids2)
-    then true else false.
-
-Fixpoint alloc_variables_c (ce: composite_env) (e: env)
-         (vars: list (ident * type))
-  : itree eff env := 
-  match vars with
-  | [] => Ret e
-  | (id, ty) :: vars' =>
-    v <- ccallU "salloc" (0%Z, sizeof ce ty);;
-    match v with
-    | Vptr b ofs => alloc_variables_c ce (PTree.set id (b, ty) e) vars'
-    | _ => triggerUB (* dummy *)
-    end
-  end.
-
-Definition function_entry_c
-           (ce: composite_env) (f: function) (vargs: list val)
-  : itree eff (env * temp_env) :=
-  if (id_list_norepet_c (var_names (fn_vars f)) &&
-      id_list_norepet_c (var_names (fn_params f)) &&
-      id_list_disjoint_c (var_names (fn_params f))
-                         (var_names (fn_temps f)))%bool
-  then
-    e <- alloc_variables_c ce empty_env (fn_vars f);;
-    le <- (bind_parameter_temps (fn_params f) vargs (create_undef_temps (fn_temps f)))?;;
-    Ret (e, le)
-  else triggerUB.
-
-Section DECOMP.
-
-  Definition runtime_env : Type := env * temp_env * option bool * option val.
-
-  Notation itr_t := (itree eff runtime_env).
-
-  Definition _sassign_c e le a1 a2 :=
-    tau;;
-    '(loc, (ofs, bf)) <- eval_lvalue_c e le a1;;
-     v2 <- eval_expr_c e le a2;; 
-     v2' <- sem_cast_c v2 (typeof a2) (typeof a1);;
-     v2' <- v2'?;;
-     assign_loc_c ce (typeof a1) loc ofs bf v2.
-
-  Definition _scall_c e le a al
-    : itree eff val :=
-    match Cop.classify_fun (typeof a) with
-    | Cop.fun_case_f tyargs tyres cconv =>
-      tau;;
-      vf <- eval_expr_c e le a;;
-      vargs <- eval_exprlist_c e le al tyargs;;
-      match vf with
-      | Vptr b ofs =>
-          '(gsym, skentry) <- (nth_error sk (pred (Pos.to_nat b)))?;;
-          `gd : globdef _ type <- (skentry↓)?;;
-          fd <- (match gd with Gfun fd => Some fd | _ => None end)?;;
-          if type_eq (type_of_fundef fd)
-               (Tfunction tyargs tyres cconv)
-          then ccallU gsym vargs
-          else triggerUB
-      | _ => triggerUB (* unreachable b*)
-      end
-    | _ => triggerUB
-    end.
-
-  Definition _site_c
-             (e: env) (le: temp_env) (a: expr)
-    : itree eff bool :=
-    tau;;
-    v1 <- eval_expr_c e le a;;
-    b <- bool_val_c v1 (typeof a);;
-    b?.
-
-  Definition sloop_iter_body_one
-             (itr: itr_t)
-    : itree eff (env * temp_env * (option (option val))) :=
-    '(e', le', obc, v) <- itr;;
-    match v with
-    | Some retv =>
-      (* return *)
-      Ret (e', le', Some (Some retv))
-    | None =>
-      if (* is_break *)
-        match obc with
-        | None => false
-        | Some bc => bc
-        end
-      then
-        (* break, not return *)
-        Ret (e', le', Some None)
-      else
-        (* continue *)
-        Ret (e', le', None)
-    end.
-
-  Definition sloop_iter_body_two
-             (itr: itr_t)
-    : itree eff (env * temp_env * (option (option val))) :=
-    '(e', le', obc, v) <- itr;;
-    match v with
-    | Some retv =>
-      (* return *)
-      Ret (e', le', Some (Some retv))
-    | None =>
-      match obc with
-      | Some true => Ret (e', le', Some None)
-      | Some false => triggerUB
-      | None => Ret (e', le', None)
-      end
-    end.
-
-  Definition sloop_iter_body
-             (itr1 itr2: env -> temp_env -> itr_t)
-             (i: env * temp_env)
-    : itree eff
-            (env * temp_env +
-             env * temp_env * option val) :=
-    let '(e, le) := i in
-    (* '(e1, le1, m1, obc1, v1) <- itr1 e le m ;; *)
-    '(e1, le1, ov1) <- sloop_iter_body_one (itr1 e le) ;;
-    match ov1 with
-    | Some v1 =>
-      (* break or return *)
-      Ret (inr (e1, le1, v1))
-    | None =>
-      (* run loop2 *)
-      '(e2, le2, ov2) <- sloop_iter_body_two (itr2 e1 le1);;
-      match ov2 with
-      | Some v2 =>
-        Ret (inr (e2, le2, v2))
-      | None =>
-        Ret (inl (e2, le2))
-      end
-    end.
-
-  Definition _sloop_itree
-             (e: env) (le: temp_env)
-             (itr1 itr2: env -> temp_env -> itr_t)
-    : itr_t :=
-    '(e', le', v) <-
-    ITree.iter (sloop_iter_body itr1 itr2) (e, le) ;;
-    Ret (e', le', None, v).
-
-  Fixpoint free_list_aux (l: list (block * Z * Z)): itree eff unit :=
-    match l with
-    | nil => Ret tt
-    | (b, lo, hi):: l' =>
-      `_ : () <- ccallU "sfree" (b, lo, hi);;
-      free_list_aux l'
-    end.
-
-  Definition block_of_binding (ce: composite_env) (id_b_ty: ident * (block * type)) :=
-    let (_, p) := id_b_ty in let (b, ty) := p in (b, 0%Z, sizeof ce ty).
-
-  Definition blocks_of_env (ce: composite_env) :=
-    List.map (block_of_binding ce) ∘ PTree.elements.
-  
-  Definition _sreturn_c
-             (retty: type)
-             (e: env) (le: temp_env)
-             (oa: option expr)
-    : itree eff val :=
-    match oa with
-    | None => Ret Vundef
-    | Some a =>
-      tau;;
-      v <- eval_expr_c e le a;;
-      v' <- sem_cast_c v (typeof a) retty;;
-      v'?
-    end.
-
-  Fixpoint decomp_stmt
-           (retty: type)
-           (stmt: statement)
-           (e: env) (le: temp_env)
-    : itr_t :=
-    match stmt with
-    | Sskip =>
-      tau;;Ret (e, le, None, None)
-    | Sassign a1 a2 =>
-      _sassign_c e le a1 a2;;;
-      Ret (e, le, None, None)
-    | Sset id a =>
-      tau;;
-      v <- eval_expr_c e le a ;;
-      let le' := PTree.set id v le in
-      Ret (e, le', None, None)
-    | Scall optid a al =>
-        v <- _scall_c e le a al;;
-        Ret (e, (set_opttemp optid v le), None, None)
-    | Sbuiltin optid ef targs el => triggerUB
-    | Ssequence s1 s2 =>
-      '(e', le', bc, v) <- decomp_stmt retty s1 e le;;
-      match v with
-      | Some retval =>
-        Ret (e', le', None, v)
-      | None =>
-        match bc with
-        | None =>
-          decomp_stmt retty s2 e' le'
-        | Some _ =>
-          Ret (e', le', bc, None)
-        end
-      end
-    | Sifthenelse a s1 s2 =>
-      b <- _site_c e le a;;
-      if (b: bool) then (decomp_stmt retty s1 e le)
-      else (decomp_stmt retty s2 e le)
-    | Sloop s1 s2 =>
-      let itr1 := decomp_stmt retty s1 in
-      let itr2 := decomp_stmt retty s2 in
-      _sloop_itree e le itr1 itr2
-    | Sbreak =>
-      Ret (e, le, Some true, None)
-    | Scontinue =>
-      Ret (e, le, Some false, None)
-    | Sreturn oa =>
-      v <- _sreturn_c retty e le oa;;
-      Ret (e, le, None, Some v)
-    | _ =>
-      (* not supported *)
-      triggerUB
-    end.
-
-  Definition decomp_func
-           (f: Clight.function)
-           (vargs: list val)
-    : itree eff val :=
-    '(e, le) <- function_entry_c ce f vargs;;
-    '(e', _, c, ov) <- decomp_stmt (fn_return f) (fn_body f) e le;; c?;;;
-    free_list_aux (blocks_of_env ce e');;;
-    match ov with
-    | None => Ret Vundef
-    | Some v => Ret v
-    end.
-
-    Lemma unfold_decomp_stmt :
-    decomp_stmt =
-  fun retty stmt e le =>
-    match stmt with
-    | Sskip =>
-      tau;;Ret (e, le, None, None)
-    | Sassign a1 a2 =>
-      _sassign_c e le a1 a2;;;
-      Ret (e, le, None, None)
-    | Sset id a =>
-      tau;;
-      v <- eval_expr_c e le a ;;
-      let le' := PTree.set id v le in
-      Ret (e, le', None, None)
-    | Scall optid a al =>
-        v <- _scall_c e le a al;;
-        Ret (e, (set_opttemp optid v le), None, None)
-    | Sbuiltin optid ef targs el => triggerUB
-    | Ssequence s1 s2 =>
-      '(e', le', bc, v) <- decomp_stmt retty s1 e le;;
-      match v with
-      | Some retval =>
-        Ret (e', le', None, v)
-      | None =>
-        match bc with
-        | None =>
-          decomp_stmt retty s2 e' le'
-        | Some _ =>
-          Ret (e', le', bc, None)
-        end
-      end
-    | Sifthenelse a s1 s2 =>
-      b <- _site_c e le a;;
-      if (b: bool) then (decomp_stmt retty s1 e le)
-      else (decomp_stmt retty s2 e le)
-    | Sloop s1 s2 =>
-      let itr1 := decomp_stmt retty s1 in
-      let itr2 := decomp_stmt retty s2 in
-      _sloop_itree e le itr1 itr2
-    | Sbreak =>
-      Ret (e, le, Some true, None)
-    | Scontinue =>
-      Ret (e, le, Some false, None)
-    | Sreturn oa =>
-      v <- _sreturn_c retty e le oa;;
-      Ret (e, le, None, Some v)
-    | _ =>
-      (* not supported *)
-      triggerUB
-    end.
-    Proof. repeat (apply func_ext; i). destruct x0; et. Qed.
-
-End DECOMP.
 End Clight.
-(* Notation call_data := (block * (* fundef * *) list val * mem)%type. *)
-
-(* Section TRANS. *)
-
-(*   (* Variable cprog_app: Clight.program. *) *)
-(*   Variable global_definitions : list (ident * globdef fundef type). *)
-(*   Variable public_idents : list ident. *)
-(*   Let defined_names := List.map fst global_definitions. *)
-
-(*   Fixpoint filter_dec_not {A: Type} {P: A -> Prop} (f: forall x: A, {P x} + {~ P x}) (l: list A) : list A := *)
-(*     match l with *)
-(*     | nil => nil *)
-(*     | x :: l' => if f x then filter_dec_not f l' else x :: (filter_dec_not f l') *)
-(*     end. *)
-  
-(*   Definition in_public x := in_dec Pos.eq_dec x public_idents. *)
-  
-(*   Definition rest_names := filter_dec_not in_public defined_names. *)
-
-(*   Definition in_rest x := in_dec Pos.eq_dec x rest_names. *)
-
-(*   Variable src_name : string.   (* source code file name *) *)
-
-(*   Definition prefix_pos pos := ident_of_string (src_name ++ "." ++ (string_of_ident pos))%string. *)
-
-(*   Definition rpl_pos pos := if in_rest pos then prefix_pos pos else pos. *)
-
-(*   Definition rpl_glob := List.map (fun x => (rpl_pos (fst x), snd x)) global_definitions. *)
-  
-(*   Fixpoint rpl_expr (e: expr) := *)
-(*     match e with *)
-(*     | Econst_int _ _ | Econst_float _ _ | Econst_single _ _ *)
-(*     | Econst_long _ _ | Etempvar _ _ | Esizeof _ _ | Ealignof _ _ => e *)
-(*     | Evar id ty => Evar (rpl_pos id) ty *)
-(*     | Ederef e' ty => Ederef (rpl_expr e') ty *)
-(*     | Eaddrof e' ty => Eaddrof (rpl_expr e') ty *)
-(*     | Eunop uop e' ty => Eunop uop (rpl_expr e') ty *)
-(*     | Ebinop bop e1 e2 ty => Ebinop bop (rpl_expr e1) (rpl_expr e2) ty *)
-(*     | Ecast e' ty => Ecast (rpl_expr e') ty *)
-(*     | Efield e' id ty => Efield (rpl_expr e') id ty *)
-(*     end. *)
-  
-(*   Fixpoint rpl_body (s : statement) := *)
-(*     match s with *)
-(*     | Sskip | Sbreak | Scontinue | Sgoto _ => s *)
-(*     | Sassign a1 a2 => Sassign (rpl_expr a1) (rpl_expr a2) *)
-(*     | Sset id a => Sset (rpl_pos id) (rpl_expr a) *)
-(*     | Scall optid a al => *)
-(*         Scall *)
-(*           (option_rec (fun _ => _) (Some ∘ rpl_pos) None optid) *)
-(*           (rpl_expr a) (List.map rpl_expr al) *)
-(*     | Sbuiltin optid ef targs el => *)
-(*         Sbuiltin *)
-(*           (option_rec (fun _ => _) (Some ∘ rpl_pos) None optid) *)
-(*           ef targs (List.map rpl_expr el) *)
-(*     | Ssequence s1 s2 => Ssequence (rpl_body s1) (rpl_body s2) *)
-(*     | Sifthenelse a s1 s2 => Sifthenelse (rpl_expr a) (rpl_body s1) (rpl_body s2) *)
-(*     | Sloop s1 s2 => Sloop (rpl_body s1) (rpl_body s2) *)
-(*     | Sreturn oa => Sreturn (option_rec (fun _ => _) (Some ∘ (rpl_expr)) None oa) *)
-(*     | Sswitch a ls => Sswitch (rpl_expr a) (rpl_labeled_stmt ls) *)
-(*     | Slabel l s => Slabel l (rpl_body s) *)
-(*     end *)
-      
-(*   with rpl_labeled_stmt (ls: labeled_statements) := *)
-(*          match ls with *)
-(*          | LSnil => LSnil *)
-(*          | LScons optz s ls' => LScons optz (rpl_body s) (rpl_labeled_stmt ls') *)
-(*          end. *)
-  
-(*   Definition trans_func (f: function) := *)
-(*     mkfunction f.(fn_return) f.(fn_callconv) f.(fn_params) f.(fn_vars) f.(fn_temps) (rpl_body f.(fn_body)). *)
-
-(*   Definition trans_initval (ii : init_data) := *)
-(*     match ii with *)
-(*     | Init_addrof id ofs => Init_addrof (rpl_pos id) ofs *)
-(*     | _ => ii *)
-(*     end. *)
-
-(*   Definition trans_var (gv: globvar type) := *)
-(*     {| *)
-(*       gvar_info := gv.(gvar_info); *)
-(*       gvar_init := List.map trans_initval gv.(gvar_init); *)
-(*       gvar_readonly := gv.(gvar_readonly); *)
-(*       gvar_volatile := gv.(gvar_volatile); *)
-(*     |} *)
-(*   . *)
-
-(*   Definition trans_global_def (g_def: globdef fundef type) := *)
-(*     match g_def with *)
-(*     | Gvar gv => Gvar (trans_var gv) *)
-(*     | Gfun (Internal f) => Gfun (Internal (trans_func f)) *)
-(*     | _ => g_def *)
-(*     end. *)
-
-
-(*   Definition trans_global_defs (g_defs: list (ident * globdef fundef type)) := *)
-(*     List.map (fun x => (rpl_pos (fst x), trans_global_def (snd x))) g_defs. *)
-
-(*   (* Program Definition append_srcname : Clight.program :=  *) *)
-(*   (*   {| *) *)
-(*   (*     prog_defs := trans_global_defs global_definitions; *) *)
-(*   (*     prog_public := public_idents; *) *)
-(*   (*     prog_main := cprog_app.(prog_main); *) *)
-(*   (*     prog_types := cprog_app.(prog_types); *) *)
-(*   (*     prog_comp_env := cprog_app.(prog_comp_env); *) *)
-(*   (*   |}. *) *)
-(*   (* Next Obligation. destruct cprog_app;auto. Qed. *) *)
-
-(* End TRANS. *)
-
-(* Section SITE_APP. *)
-(*   (* for site specific execution *) *)
-(*   (* not for proof *) *)
-(*   Import EventsL. *)
-
-(*   Definition sname := string. *)
-(*   Variable sn: sname. *)
-(*   Variable shared_fun_list: list gname. *)
-
-(*   Let is_shared_fun fn := in_dec string_dec fn shared_fun_list. *)
-
-(*   Definition site_append_morph_1 : Es ~> Es. (* for site specific module *) *)
-(*   Proof. *)
-(*     intros. destruct X. *)
-(*     { destruct c. destruct (is_shared_fun fn). *)
-(*       - exact (inl1 (Call mn fn args)). *)
-(*       - exact (inl1 (Call mn (sn ++ "." ++ fn) args)). } *)
-(*     destruct s. *)
-(*     { destruct s. *)
-(*       { destruct (is_shared_fun fn). *)
-(*         - exact (inr1 (inl1 (Spawn fn args))). *)
-(*         - exact (inr1 (inl1 (Spawn (sn ++ "." ++ fn) args))). } *)
-(*       exact (inr1 (inl1 Yield)). *)
-(*       exact (inr1 (inl1 Getpid)). *)
-(*       exact (inr1 (inl1 Getsn)). } *)
-(*     destruct s. *)
-(*     { destruct p. *)
-(*       - exact (inr1 (inr1 (inl1 (PPut (sn ++ "." ++ mn) p)))). *)
-(*       - exact (inr1 (inr1 (inl1 (PGet (sn ++ "." ++ mn))))). } *)
-(*     { destruct e. *)
-(*       exact (inr1 (inr1 (inr1 (Choose X)))). *)
-(*       exact (inr1 (inr1 (inr1 (Take X)))). *)
-(*       exact (inr1 (inr1 (inr1 (Syscall fn args rvs)))). } *)
-(*   Defined. *)
-  
-(*   Definition site_append_morph_2 (sn': sname) : Es ~> Es. (* for shared module *) *)
-(*   Proof. *)
-(*     intros. destruct X. *)
-(*     { destruct c. destruct (is_shared_fun fn). *)
-(*       - exact (inl1 (Call mn fn args)). *)
-(*       - exact (inl1 (Call mn (sn' ++ "." ++ fn) args)). } *)
-(*     destruct s. *)
-(*     { destruct s. *)
-(*       { destruct (is_shared_fun fn). *)
-(*         - exact (inr1 (inl1 (Spawn fn args))). *)
-(*         - exact (inr1 (inl1 (Spawn (sn' ++ "." ++ fn) args))). } *)
-(*       exact (inr1 (inl1 Yield)). *)
-(*       exact (inr1 (inl1 Getpid)). *)
-(*       exact (inr1 (inl1 Getsn)). *)
-(*     } *)
-(*     destruct s. *)
-(*     { destruct p. *)
-(*       - exact (inr1 (inr1 (inl1 (PPut mn p)))). *)
-(*       - exact (inr1 (inr1 (inl1 (PGet mn)))). } *)
-(*     { destruct e. *)
-(*       exact (inr1 (inr1 (inr1 (Choose X)))). *)
-(*       exact (inr1 (inr1 (inr1 (Take X)))). *)
-(*       exact (inr1 (inr1 (inr1 (Syscall fn args rvs)))). } *)
-(*   Defined. *)
-    
-
-(*   Definition site_appended_itree_1 : itree Es ~> itree Es := translate site_append_morph_1. *)
-(*   Definition site_appended_itree_2 (sn': sname) : itree Es ~> itree Es := translate (site_append_morph_2 sn'). *)
-
-(*   Definition append_site_1 (ms: ModSemL.t) : ModSemL.t := *)
-(*     {| *)
-(*       ModSemL.fnsems := List.map (fun '(gn, fnsem) => *)
-(*                        ((sn ++ "." ++ gn)%string, fun x => site_appended_itree_1 _ (fnsem x))) ms.(ModSemL.fnsems); *)
-(*       ModSemL.initial_mrs := List.map (map_fst (fun mn => (sn ++ "." ++ mn)%string)) ms.(ModSemL.initial_mrs); *)
-(*     |} *)
-(*   . *)
-
-(*   Definition append_caller_site {X Y: Type} (body: X -> itree Es Y) := *)
-(*     fun x => sn' <- trigger Getsn;; site_appended_itree_2 sn' _ (body x). *)
-
-(*   Definition append_site_2 (ms: ModSemL.t) : ModSemL.t := *)
-(*     {| *)
-(*       ModSemL.fnsems := List.map *)
-(*                           (fun '(gn, fnsem) => (gn, append_caller_site fnsem)) ms.(ModSemL.fnsems); *)
-(*       ModSemL.initial_mrs := ms.(ModSemL.initial_mrs); *)
-(*     |} *)
-(*   . *)
-
-(* End SITE_APP. *)
-
-
-Section DECOMP_PROG.
-
-  (* Context `{SystemEnv}. *)
-  Variable types: list composite_definition.
-  Variable defs: list (ident * globdef Clight.fundef type).
-  Variable public: list ident.
-  Variable wf: wf_composites types.
-  Let ce: composite_env := let (ce, _) := build_composite_env' types wf in ce.
-  
-  Variable mn: string.
-
-  (* Fixpoint get_source_name (filename : string) := *)
-  (*   String.substring 0 (String.length filename - 2) filename. *)
-
-  Fixpoint decomp_fundefs (sk: Sk.t)
-           (defs: list (ident * globdef Clight.fundef type))
-    : list (ident * (list val -> itree Es val)) :=
-    match defs with
-    | [] => []
-    | (id, gdef) :: defs' =>
-      match gdef with
-      | Gvar _ => decomp_fundefs sk defs'
-      | Gfun fd =>
-        match fd with
-        | Internal f => 
-          (id, fun vl => 
-                  v <- decomp_func sk ce f vl;; 
-                  (if Pos.eq_dec id (ident_of_string "main")
-                   then (match v with Vint _ => Ret v | _ => triggerUB end)
-                   else Ret v)) :: decomp_fundefs sk defs'
-        | _ => decomp_fundefs sk defs'
-        end
-      end
-    end.
-
-  Fixpoint get_sk (defs: list (ident * globdef Clight.fundef type)) :=
-    match defs with
-    | [] => []
-    | (id, gdef) :: defs' =>
-        match gdef with
-        | Gvar gv => (string_of_ident id, gdef↑) :: get_sk defs'
-        | Gfun gf =>
-            match gf with
-            | Internal f => (string_of_ident id, gdef↑) :: get_sk defs'
-            | _ => get_sk defs'
-            end
-        end
-    end
-  .
-
-  Definition modsem (sk: Sk.t) : ModSem.t := {|
-    ModSem.fnsems := List.map (fun '(fn, f) => (string_of_ident fn, cfunU f)) (decomp_fundefs sk defs);
-    ModSem.mn := mn;
-    ModSem.initial_st := tt↑;
-  |}.
-
-  Definition get_mod : Mod.t := {|
-    Mod.get_modsem := modsem;
-    Mod.sk := get_sk defs;
-  |}.
-
-End DECOMP_PROG.
-
-(* Section EXECUTION_STRUCTURE. *)
-(*   (*   execution modules consist of modules executes in sites independently  *) *)
-(*   (*   and modules accessable in every sites. *) *)
-(*   (* ------------------------------------------------------------------------ *) *)
-(*   (* example *) *)
-(*   (* site A : A1 A2 A3 *) *)
-(*   (* site B : B1 B2 B3 *) *)
-(*   (* shared : C1 C2 C3 *) *)
-(*   (* f: function append site name in local state and its own function *) *)
-(*   (* g: function append current site name in site specific function (so, its site name dynamically determined) *) *)
-(*   (* A's ModSemL: f (MemA + A1 + A2 + A3) <_ (enclose) skel of site A and shared *) *)
-(*   (* B's ModSemL: f (MemB + B1 + B2 + B3) <_ (enclose) skel of site B and shared *) *)
-(*   (* shared's ModSemL: g (C1 + C2 + C3) <_(enclose) skel of site A and site B and shared *) *)
-
-(*   Fixpoint remove_mult_name (l : Sk.t) : Sk.t := *)
-(*     match l with *)
-(*       | [] => [] *)
-(*       | (gn, gd)::xs => if in_dec string_dec gn (List.map fst xs) then remove_mult_name xs else (gn, gd)::(remove_mult_name xs) *)
-(*     end. *)
-
-(*   (* for skeleton padding *) *)
-(*   Definition sk_padmod (sk: Sk.t) := ModL.mk ModL.empty.(ModL.get_modsem) sk. *)
-
-(*   (* get one site's ModSemL *) *)
-(*   Definition proc_gen (shared_module: ModL.t) : sname * list Mod.t -> ModSemL.t := *)
-(*     fun '(sn, modlist) => *)
-(*       (append_site_1 sn (List.map fst shared_module.(ModL.enclose).(ModSemL.fnsems)) *)
-(*          (ModL.enclose (ModL.add (Mod.add_list modlist) (sk_padmod shared_module.(ModL.sk))))). *)
-  
-(*   (* turns exec_profile into one ModSemL *) *)
-(*   Definition sum_of_site_modules_view (exec_profile: list (sname * list Mod.t)) (shared_module: ModL.t) : ModSemL.t := *)
-(*     List.fold_left ModSemL.add (List.map (proc_gen shared_module) exec_profile) (ModSemL.mk [] []). *)
-
-(*   (* get all skeletons in sites and concat *) *)
-(*   Definition sum_of_site_skeletons (exec_profile: list (sname * list Mod.t)) : Sk.t := *)
-(*       remove_mult_name (List.concat (List.map (fun '(sn, modlist) => (Mod.add_list modlist).(ModL.sk)) exec_profile)). *)
-
-(*   (* turn shared modules into one ModSemL *) *)
-(*   Definition view_shared_module (exec_profile: list (sname * list Mod.t)) (shared_module: ModL.t) : ModSemL.t := *)
-(*     append_site_2 (List.map fst shared_module.(ModL.enclose).(ModSemL.fnsems)) *)
-(*       (ModL.enclose (ModL.add shared_module (sk_padmod (sum_of_site_skeletons exec_profile)))). *)
-  
-(* End EXECUTION_STRUCTURE. *)
