clightlight/Clightlight2ClightGenv.v
@@ -9,7 +9,7 @@ Require Import Any.
 Require Import ModSem.
 Require Import AList.
 
-Require Import ConvC2ITree.
+Require Import ConvC2ITreeStmt.
 Require Import Clightlight2ClightMatch.
 
 From compcert Require Import Ctypes Clight Clightdefs.
