clightlight/Clightlight2ClightLenv.v
@@ -13,10 +13,10 @@ Section LENV.
   Context `{Σ: GRA.t}.
   Context `{builtins : builtinsTy}.
 
-  Lemma match_update_le defs le tle o v
-        (MLE: match_le defs le tle)
+  Lemma match_update_le sk defs le tle o v
+        (MLE: match_le sk defs le tle)
     :
-      match_le defs (set_opttemp o v le) (set_opttemp o (map_val defs v) tle).
+      match_le sk defs (set_opttemp o v le) (set_opttemp o (map_val sk defs v) tle).
   Proof.
     destruct o; ss. econs. i. inv MLE. destruct (Pos.eq_dec i id).
     - subst. rewrite PTree.gss in *. clarify.
@@ -24,11 +24,11 @@ Section LENV.
   Qed.
 
   Lemma update_le
-        defs x id v sv le tle
+        sk defs x id v sv le tle
         (SRC_UPDATE: Maps.PTree.get x (Maps.PTree.set id v tle) = Some sv)
-        (MLE: match_le defs le tle)
+        (MLE: match_le sk defs le tle)
     :
-      Maps.PTree.get x (Maps.PTree.set id (map_val defs v) tle) = Some (map_val defs sv).
+      Maps.PTree.get x (Maps.PTree.set id (map_val sk defs v) tle) = Some (map_val sk defs sv).
   Proof.
   Admitted.
 
@@ -44,10 +44,10 @@ Section LENV.
   Qed.
 
   Lemma bind_parameter_temps_exists
-        defs base params sle rvs (tle0: temp_env)
+        sk defs base params sle rvs (tle0: temp_env)
         (BIND_SRC: bind_parameter_temps params rvs base = Some sle)
     :
-      exists tle, (<<BIND_TGT: bind_parameter_temps params (List.map (map_val defs) rvs) tle0
+      exists tle, (<<BIND_TGT: bind_parameter_temps params (List.map (map_val sk defs) rvs) tle0
                       = Some tle>>).
   Proof.
     eapply bind_parameter_temps_exists_if_same_length; eauto.
