clightlight/Clightlight2ClightMatchStmt.v
@@ -1,0 +1,224 @@
+From compcert Require Import Globalenvs Smallstep AST Integers Events Behaviors Errors Memory Values Maps.
+Require Import Coqlib.
+Require Import ITreelib.
+Require Import Skeleton.
+Require Import PCM.
+Require Import STS Behavior.
+Require Import Any.
+Require Import ModSem.
+Require Import ConvC2ITree.
+Require Import ConvC2ITreeStmt.
+Require Import Clight_Mem0.
+
+Set Implicit Arguments.
+
+From compcert Require Import Ctypes Clight Clightdefs Globalenvs.
+
+Require Import Clightlight2ClightMatch.
+
+Import Genv.
+
+Section MATCH.
+
+  Context `{Σ: GRA.t}.
+  
+  Import List.
+
+  Local Open Scope Z.
+
+  (* global env is fixed when src program is fixed *)
+  Variable sk : Sk.t.
+  Variable tge : Genv.t Clight.fundef type.
+
+  (* composite env should be fixed when src program is fixed*)
+  Variable ce : composite_env.
+
+  (* ModSem should be fixed with src too *)
+  Variable ms : ModSemL.t.
+
+  Definition itr_t := itree Es runtime_env.
+
+  (* clightlight state should be expressed by two constructs, stmt and cont *)
+  Definition clightlight_state := itree eventE Any.t.
+
+  Definition Es_to_eventE {A} (ms: ModSemL.t) (mn: string) (es_itree: itree Es A) (rp: p_state) :=
+     EventsL.interp_Es (ModSemL.prog ms) (transl_all mn es_itree) rp.
+
+  Definition itree_of_code (mn: string) (retty: type) (code: statement) (e: env) (le: temp_env) 
+    : stateT p_state (itree eventE) runtime_env 
+      := Es_to_eventE ms mn (decomp_stmt sk ce retty code e le).
+
+  Definition ktree_of_cont_itree (mn: string) (cont_itr: runtime_env -> itr_t)
+    : p_state * runtime_env -> itree eventE (p_state * runtime_env) 
+      := fun '(pstate, ncr) => Es_to_eventE ms mn (cont_itr ncr) pstate.
+
+  Definition itree_of_cont_pop (itr_sreturn: itr_t) (itr_sbreak: itr_t) (itr_scontinue: itr_t) (itr_skip: itr_t) 
+  : option bool -> option val -> itr_t :=
+    fun optb optv =>
+      match optv with
+      | Some _ => itr_sreturn
+      | None =>
+        match optb with
+        | Some true => itr_sbreak
+        | Some false => itr_scontinue
+        | None => itr_skip
+        end
+      end.
+
+  Definition kstop_itree (ncr: runtime_env) : itree Es val := 
+    let '(e, le, optb, optv) := ncr in
+      '(_, _, _, optv') <- (itree_of_cont_pop 
+                              (free_list_aux (ConvC2ITreeStmt.blocks_of_env ce e);;; Ret (e, le, None, optv)) 
+                              triggerUB 
+                              triggerUB 
+                              triggerUB) optb optv;; 
+      v <- optv'?;; (match v with | Vint _ => Ret v | _ => triggerUB end).
+
+  Definition itree_stop (mn: string) := fun '(pstate, ncr) => Es_to_eventE ms mn (kstop_itree ncr) pstate.
+
+    (* below is functional version of continuation translation *)
+    (*
+  Fixpoint decomp_cont (retty: type) (k: Clight.cont) (e: env) (le: temp_env) (optb: option bool) (optv: option val) : itree eff val :=
+    match k with
+    | Kseq code k' => 
+      '(e', le', optb', optv') <- (treat_flow 
+                                    (Ret (e, le, None, optv)) 
+                                    (Ret (e, le, optb, None)) 
+                                    (Ret (e, le, optb, None)) 
+                                    (decomp_stmt retty code e le)) optb optv;;
+      decomp_cont retty k' e' le' optb' optv'
+    | Kloop1 code1 code2 k' => 
+      '(e', le', optb', optv') <- (treat_flow 
+                                    (Ret (e, le, None, optv)) 
+                                    (Ret (e, le, None, None)) 
+                                    ('(e2, le2, ov2) <- sloop_iter_body_two (decomp_stmt retty code2 e le);;
+                                     match ov2 with
+                                     | Some v2 => Ret (e2, le2, None, v2)
+                                     | None => _sloop_itree e2 le2 (decomp_stmt retty code1) (decomp_stmt retty code2)
+                                     end)
+                                    ('(e2, le2, ov2) <- sloop_iter_body_two (decomp_stmt retty code2 e le);;
+                                     match ov2 with
+                                     | Some v2 => Ret (e2, le2, None, v2)
+                                     | None => _sloop_itree e2 le2 (decomp_stmt retty code1) (decomp_stmt retty code2)
+                                     end)) optb optv;;
+      decomp_cont retty k' e' le' optb' optv'
+    | Kloop2 code1 code2 k' =>
+      '(e, le, ov2) <- (match optv with 
+                        | Some v => Ret (e, le, Some (Some v)) 
+                        | None => 
+                          match optb with 
+                          | Some true => Ret (e, le, Some None)
+                          | Some false => triggerUB
+                          | None => Ret (e, le, None)
+                          end
+                        end);;
+      '(e', le', optb', optv') <- (match ov2 with
+                                  | Some v2 => Ret (e, le, None, v2)
+                                  | None => _sloop_itree e le (decomp_stmt retty code1) (decomp_stmt retty code2)
+                                  end);;
+      decomp_cont retty k' e' le' optb' optv'
+    | Kstop => 
+      '(_, _, _, optv') <- (treat_flow 
+                            (free_list_aux (blocks_of_env ce e);;; Ret (e, le, None, optv)) 
+                            triggerUB 
+                            triggerUB 
+                            triggerUB) optb optv;;
+      v <- optv'?;; (match v with Vint _ => Ret v | _ => triggerUB end)
+    | Kcall optid f e' le' k' =>
+      '(_, _, _, optv') <- (treat_flow 
+                            (free_list_aux (blocks_of_env ce e);;; tau;; Ret (e, le, None, optv)) 
+                            triggerUB 
+                            triggerUB 
+                            (free_list_aux (blocks_of_env ce e);;; tau;; Ret (e, le, None, Some Vundef))) optb optv;;
+      v <- optv'?;; decomp_cont f.(fn_return) k' e' (set_opttemp optid v le') None None
+    | _ => triggerUB
+    end.
+     *)
+
+(* mname is just module name pops the continuation *)
+  Inductive match_cont : type -> mname -> (p_state * runtime_env -> itree eventE (p_state * val)) -> cont -> Prop := 
+  | match_cont_Kseq cont_itree next code cont retty mn
+      (ITR: cont_itree = ktree_of_cont_itree mn 
+                        (fun '(e, le, optb, optv) => 
+                          (itree_of_cont_pop
+                            (Ret (e, le, None, optv)) 
+                            (Ret (e, le, optb, None)) 
+                            (Ret (e, le, optb, None)) 
+                            (decomp_stmt sk ce retty code e le)) optb optv))
+      (NEXT: match_cont retty mn next cont)
+    :
+      match_cont retty mn (fun x => y <- cont_itree x;; next y) (Kseq code cont)
+  | match_cont_Kloop1 cont_itree next code1 code2 cont retty mn
+      (ITR: cont_itree = ktree_of_cont_itree mn
+                        (fun '(e, le, optb, optv) => 
+                          (itree_of_cont_pop
+                            (Ret (e, le, None, optv)) 
+                            (Ret (e, le, None, None)) 
+                            ('(e2, le2, ov2) <- sloop_iter_body_two (decomp_stmt sk ce retty code2 e le);;
+                              match ov2 with
+                              | Some v2 => Ret (e2, le2, None, v2)
+                              | None => _sloop_itree e2 le2 (decomp_stmt sk ce retty code1) (decomp_stmt sk ce retty code2)
+                              end)
+                            ('(e2, le2, ov2) <- sloop_iter_body_two (decomp_stmt sk ce retty code2 e le);;
+                              match ov2 with
+                              | Some v2 => Ret (e2, le2, None, v2)
+                              | None => _sloop_itree e2 le2 (decomp_stmt sk ce retty code1) (decomp_stmt sk ce retty code2)
+                              end)) optb optv))
+      (NEXT: match_cont retty mn next cont) 
+    :
+      match_cont retty mn (fun x => y <- cont_itree x;; next y) (Kloop1 code1 code2 cont)
+  | match_cont_Kloop2 cont_itree next code1 code2 cont retty mn
+      (ITR: cont_itree = ktree_of_cont_itree mn
+                        (fun '(e, le, optb, optv) => 
+                          '(e, le, ov2) <- 
+                            (match optv with 
+                            | Some v => Ret (e, le, Some (Some v)) 
+                            | None => match optb with 
+                                      | Some true => Ret (e, le, Some None)
+                                      | Some false => triggerUB
+                                      | None => Ret (e, le, None)
+                                      end
+                            end);;
+                          match ov2 with
+                          | Some v2 => Ret (e, le, None, v2)
+                          | None => _sloop_itree e le (decomp_stmt sk ce retty code1) (decomp_stmt sk ce retty code2)
+                          end))
+      (NEXT: match_cont retty mn next cont) 
+    :
+      match_cont retty mn (fun x => y <- cont_itree x;; next y) (Kloop2 code1 code2 cont)
+  | match_cont_Kstop cont_itree retty mn
+      (ITR: cont_itree = itree_stop mn)
+    :
+      match_cont retty mn cont_itree Kstop
+  | match_cont_Kcall cont_itree next optid f e' le' te' tle' cont retty mn_caller mn_callee
+      (ITR: cont_itree = ktree_of_cont_itree mn_callee
+                        (fun '(e, le, optb, optv) => 
+                          '(_, _, _, optv') <-
+                            (itree_of_cont_pop
+                              (free_list_aux (ConvC2ITreeStmt.blocks_of_env ce e);;; tau;; Ret (e, le, None, optv)) 
+                              triggerUB 
+                              triggerUB 
+                              (free_list_aux (ConvC2ITreeStmt.blocks_of_env ce e);;; tau;; Ret (e, le, None, Some Vundef))) optb optv;;
+                          v <- optv'?;; Ret (e', set_opttemp optid v le', None, None))) 
+      (CONT_ENV_MATCH: match_e sk tge e' te')
+      (CONT_LENV_MATCH: match_le sk tge le' tle')
+      (NEXT: match_cont f.(fn_return) mn_caller next cont) 
+    :
+      match_cont retty mn_callee (fun x => y <- cont_itree x;; next y) (Kcall optid f te' tle' cont).
+  
+
+  Variant match_states : itree eventE Any.t -> Clight.state -> Prop :=
+  | match_states_intro
+      tf pstate e te le tle tcode m tm tcont mn itr_code itr_cont itr
+      (MGE: match_ge sk tge)
+      (ME: match_e sk tge e te)
+      (ML: match_le sk tge le tle)
+      (PSTATE: pstate "Mem"%string = m↑)
+      (MM: match_mem sk tge m tm)
+      (MCODE: itr_code = itree_of_code mn tf.(fn_return) tcode e le pstate)
+      (MCONT: match_cont tf.(fn_return) mn itr_cont tcont)
+      (MENTIRE: itr = x <- itr_code;; '(_, v) <- itr_cont x;; Ret v↑)
+    :
+      match_states itr (State tf tcode tcont te tle tm)
+  .
+End MATCH.
