clightlight/Clightlight2ClightSimAll.v
@@ -1,0 +1,278 @@
+From compcert Require Import Globalenvs Smallstep AST Integers Events Behaviors Errors Memory.
+Require Import Coqlib.
+Require Import ITreelib.
+Require Import Skeleton.
+Require Import PCM.
+Require Import STS Behavior.
+Require Import Any.
+Require Import ModSem.
+Require Import ConvC2ITree.
+Require Import ConvC2ITreeStmt.
+Require Import SimSTS3.
+Require Import Clight_Mem0.
+Require Import IRed.
+From Ordinal Require Import Ordinal Arithmetic.
+
+Require Import Clightlight2ClightMatch.
+Require Import Clightlight2ClightArith.
+Require Import Clightlight2ClightGenv.
+Require Import Clightlight2ClightLenv.
+Require Import Clightlight2ClightMem.
+Require Import Clightlight2ClightSim.
+
+From compcert Require Import Ctypes Clight Clightdefs Values.
+
+Section PROOF.
+
+  Import ModSemL.
+
+  Context `{Σ: GRA.t}.
+  Context `{builtins : builtinsTy}.
+
+  Let _sim_mon := Eval simpl in (fun (src: ModL.t) (tgt: Clight.program) => @sim_mon (compile_val src) (Clight.semantics2 tgt)).
+  Hint Resolve _sim_mon: paco.
+
+  Ltac sim_red := try red; Red.prw ltac:(_red_gen) 2 0.
+  Ltac sim_tau := (try sim_red); pfold; econs 3; ss; clarify; eexists; exists (step_tau _); left.
+
+  Opaque arrow.
+
+  Opaque oeq. 
+
+  Ltac to_oeq :=
+    match goal with
+| |- ?A = ?B => change (oeq A B)
+    end.
+
+  Ltac from_oeq :=
+    match goal with
+    | |- oeq ?A ?B => change (A = B)
+    end.
+
+  Ltac sim_redE :=
+    to_oeq; cbn; repeat (Red.prw ltac:(_red_gen) 1 0); repeat (Red.prw ltac:(_red_gen) 2 0); from_oeq.
+
+  Ltac to_arrow :=
+    match goal with
+| |- ?A -> ?B => change (arrow A B)
+    end.
+
+  Ltac from_arrow :=
+    match goal with
+    | |- arrow ?A ?B => change (A -> B)
+    end.
+  Ltac sim_redH H :=
+    revert H; to_arrow; (repeat (cbn; Red.prw ltac:(_red_gen) 2 2 0)); from_arrow; intros H.
+
+  Ltac solve_ub := des; irw in H; dependent destruction H; clarify.
+  Ltac sim_triggerUB := 
+    (try rename H into HH); ss; unfold triggerUB; try sim_red; pfold; econs 5; i; ss; auto;
+                        [solve_ub | irw in  STEP; dependent destruction STEP; clarify].
+
+  Ltac tgt_step := pfold; econs 4; eexists; eexists; [|left].
+
+  Ltac wrap_up := pfold; econs 7; et; right.
+
+  Ltac remove_UBcase := des_ifs; try sim_red; try sim_triggerUB.
+
+  Ltac dtm H H0 := eapply angelic_step in H; eapply angelic_step in H0; des; rewrite H; rewrite H0; ss.
+
+  Local Opaque Pos.of_nat.
+
+  Local Opaque Pos.of_succ_nat.
+
+
+
+  (**** At the moment, it suffices to support integer IO in our scenario,
+        and we simplify all the other aspects.
+        e.g., the system calls that we are aware of
+        (1) behaves irrelevant from Senv.t,
+        (2) does not allow arguments/return values other than integers,
+        (3) produces exactly one event (already in CompCert; see: ec_trace_length),
+        (4) does not change memory,
+        (5) always returns without stuck,
+        and (6) we also assume that it refines our notion of system call.
+   ****)
+  Axiom syscall_exists: forall fn sg se args_tgt m0, exists tr ret_tgt m1,
+        <<TGT: external_functions_sem fn sg se args_tgt m0 tr ret_tgt m1>>
+  .
+  Axiom syscall_refines:
+    forall fn sg args_tgt ret_tgt
+           se m0 tr m1
+           (TGT: external_functions_sem fn sg se args_tgt m0 tr ret_tgt m1)
+    ,
+      exists args_int ret_int ev,
+        (<<ARGS: args_tgt = (List.map Values.Vlong args_int)>>) /\
+        (<<RET: ret_tgt = (Values.Vlong ret_int)>>) /\
+        let args_src := List.map Int64.signed args_int in
+        let ret_src := Int64.signed ret_int in
+        (<<EV: tr = [ev] /\ decompile_event ev = Some (event_sys fn args_src↑ ret_src↑)>>)
+        /\ (<<SRC: syscall_sem (event_sys fn args_src↑ ret_src↑)>>)
+        /\ (<<MEM: m0 = m1>>)
+  .
+
+  Lemma step_freeing_stack cprog f_table modl r b1 b2 ktr tstate ge ce e pstate mn (PSTATE: exists m: mem, pstate "Mem"%string = m↑) (EQ: ce = ge.(genv_cenv)) (EQ2: f_table = (ModL.add Mem modl).(ModL.enclose)) :
+  paco4
+    (_sim (ModL.compile (ModL.add Mem modl)) (semantics2 cprog)) r (match (blocks_of_env ge e) with [] => b1 | _ => true end) b2
+    (m <- (pstate "Mem")↓?;; m <- (Mem.free_list m (blocks_of_env ge e))?;; ktr (update pstate "Mem" m↑, ()))
+    tstate
+  ->
+  paco4
+    (_sim (ModL.compile (ModL.add Mem modl)) (semantics2 cprog)) r b1 b2
+    (`r0: (p_state * ()) <- 
+      (EventsL.interp_Es (prog f_table)
+        (transl_all mn (free_list_aux (ConvC2ITree.blocks_of_env ce e))) 
+        pstate)
+      ;; ktr r0) 
+    tstate.
+  Proof.
+    rewrite EQ. rewrite EQ2. clear EQ ce EQ2 f_table. des. replace (ConvC2ITree.blocks_of_env ge e) with (blocks_of_env ge e) by auto.
+    set (blocks_of_env _ _) as l. clearbody l. depgen m. depgen pstate. depgen b1. depgen b2. induction l.
+    - i. rewrite PSTATE in H. rewrite Any.upcast_downcast in H. ss. sim_red. sim_redH H.
+      replace (update pstate _ _) with pstate in H; et.
+      apply func_ext. i. s. unfold update. des_ifs.
+    - i. rewrite PSTATE in H. sim_redH H. des_ifs_safe. unfold ccallU. sim_tau.
+      des_ifs_safe. unfold sfreeF. repeat sim_tau. rewrite PSTATE. sim_red. 
+      destruct (Mem.free _) eqn: E1 in H; try (unfold unwrapU in *; des_ifs_safe; sim_triggerUB; fail).
+      rewrite E1. sim_red. repeat sim_tau. sim_red. eapply IHl; ss.
+      unfold update at 1. ss. sim_red. destruct (Mem.free_list _) eqn: E2.
+      { sim_red. sim_redH H. des_ifs; replace (update (update _ _ _) _ _) with (update pstate "Mem" (Any.upcast m1)); et.
+        all : apply func_ext; i; unfold update; des_ifs. }
+      unfold unwrapU. unfold triggerUB. sim_red. sim_triggerUB.
+  Qed.
+
+
+  Arguments Es_to_eventE /.
+  Arguments itree_of_code /. 
+  Arguments sloop_iter_body_two /. 
+  Arguments ktree_of_cont_itree /. 
+
+  Theorem match_states_sim
+          types sk defs WF_TYPES mn
+          (modl: ModL.t) ms
+          clight_prog ist cst
+          (MODL: modl = ModL.add (Mod.lift Mem) (Mod.lift (get_mod types defs WF_TYPES mn)))
+          (MODSEML: ms = modl.(ModL.enclose))
+          (TGT: clight_prog = mkprogram types defs (List.map (fun '(gn, _) => gn) defs) (ident_of_string "main") WF_TYPES)
+          (MS: match_states sk (Genv.globalenv clight_prog) (Ctypes.prog_comp_env clight_prog) ms ist cst)
+  :
+      <<SIM: sim (@ModL.compile _ EMSConfigC modl) (Clight.semantics2 clight_prog) false false ist cst>>.
+  Proof.
+    red. red.
+    depgen ist. depgen cst. pcofix CIH. i.
+    inv MS. unfold mkprogram in *. des_ifs_safe.
+    set (Genv.globalenv _) as tge in MGE. set {| genv_genv := tge; genv_cenv := x|} as ge.
+    destruct tcode.
+    - ss. sim_red. sim_tau. sim_red.
+      destruct tcont; inv MCONT; ss; clarify.
+      { sim_red. sim_triggerUB. }
+      { sim_red. tgt_step; [econs|]. wrap_up. apply CIH. econs; et. }
+      { sim_red. tgt_step; [econs; et|]. wrap_up. apply CIH. econs; et. { econs; et. } sim_redE.
+        erewrite bind_extk; et. i. des_ifs_safe. repeat (des_ifs; sim_redE; try reflexivity). }
+      { sim_red. tgt_step; [econs; et|]. wrap_up. apply CIH. econs; et. }
+      { sim_red. eapply step_freeing_stack with (ge := ge); et. 
+        rewrite PSTATE. sim_red. unfold unwrapU in *.
+        destruct (Mem.free_list m _) eqn: STACK_FREE; try sim_triggerUB.
+        inv ME. hexploit match_mem_free_list; et. i. des. 
+        sim_red. tgt_step. 
+        { econs; unfold is_call_cont; et. unfold semantics2, globalenv. ss.
+          rewrite <- TMEM. f_equal. replace _ with ge by et. 
+          set (fun _ => _) as g. clear - ME0.  
+          unfold blocks_of_env, block_of_binding.
+          rewrite ME0.
+          set (fun id_b_ty : _ * (_ * _) => _) as f.
+          set (map_env_entry _ _) as h.
+          rewrite List.map_map with (f := f).
+          replace (g ∘ f) with (f ∘ h); try rewrite List.map_map; et.
+          unfold f, g, h. apply func_ext. i. des_ifs_safe. ss. clarify. }
+        tgt_step; [econs|]. pfold. econs 7;[|des_ifs|];et. right. eapply CIH.
+        econs. 5: apply MM_POST. all: et. 
+        { hexploit match_update_le; et. instantiate (2 := Vundef). ss. et. }  
+        { instantiate (1 := update pstate "Mem" (Any.upcast m0)). ss. }
+        { et. ss. sim_redE. f_equal. f_equal. sim_redE. et. } }
+    - ss. unfold _sassign_c. sim_red. sim_tau. sim_red.
+      eapply step_eval_lvalue with (ge := ge); et. i. subst. sim_red. 
+      eapply step_eval_expr with (ge := ge); et. i. subst. sim_red. 
+      eapply step_sem_cast; et. i.
+      unfold unwrapU. des_ifs; try sim_red; try sim_triggerUB.
+      eapply step_assign_loc; et. i. sim_red.
+      tgt_step. { econs; et. } wrap_up. eapply CIH. 
+      econs. 4:{ instantiate (2 := update pstate "Mem" m'↑). unfold update. ss. } 
+      all: et. ss. sim_redE. f_equal.
+    -
+  Admitted.
+
+
+  (* Ltac rewriter :=
+    try match goal with
+        | H: _ = _ |- _ => rewrite H in *; clarify
+        end.
+
+  Lemma Csharpminor_eval_expr_determ a
+    :
+      forall v0 v1 ge e le m
+             (EXPR0: eval_expr ge e le m a v0)
+             (EXPR1: eval_expr ge e le m a v1),
+        v0 = v1.
+  Proof.
+    induction a; i; inv EXPR0; inv EXPR1; rewriter.
+    { inv H0; inv H1; rewriter. }
+    { exploit (IHa v2 v3); et. i. subst. rewriter. }
+    { exploit (IHa1 v2 v4); et. i. subst.
+      exploit (IHa2 v3 v5); et. i. subst. rewriter. }
+    { exploit (IHa v2 v3); et. i. subst. rewriter. }
+  Qed.
+
+  Lemma Csharpminor_eval_exprlist_determ a
+    :
+      forall v0 v1 ge e le m
+             (EXPR0: eval_exprlist ge e le m a v0)
+             (EXPR1: eval_exprlist ge e le m a v1),
+        v0 = v1.
+  Proof.
+    induction a; ss.
+    { i. inv EXPR0. inv EXPR1. auto. }
+    { i. inv EXPR0. inv EXPR1.
+      hexploit (@Csharpminor_eval_expr_determ a v2 v0); et. i.
+      hexploit (IHa vl vl0); et. i. clarify. }
+  Qed.
+
+  Lemma alloc_variables_determ vars
+    :
+      forall e0 e1 ee m m0 m1
+             (ALLOC0: alloc_variables ee m vars e0 m0)
+             (ALLOC1: alloc_variables ee m vars e1 m1),
+        e0 = e1 /\ m0 = m1.
+  Proof.
+    induction vars; et.
+    { i. inv ALLOC0; inv ALLOC1; auto. }
+    { i. inv ALLOC0; inv ALLOC1; auto. rewriter.
+      eapply IHvars; et. }
+  Qed.
+
+  Lemma Csharpminor_wf_semantics prog
+    :
+      wf_semantics (Csharpminor.semantics prog).
+  Proof.
+    econs.
+    { i. inv STEP0; inv STEP1; ss; rewriter.
+      { hexploit (@Csharpminor_eval_expr_determ a v v0); et. i. rewriter. }
+      { hexploit (@Csharpminor_eval_expr_determ addr vaddr vaddr0); et. i. rewriter.
+        hexploit (@Csharpminor_eval_expr_determ a v v0); et. i. rewriter. }
+      { hexploit (@Csharpminor_eval_expr_determ a vf vf0); et. i. rewriter.
+        hexploit (@Csharpminor_eval_exprlist_determ bl vargs vargs0); et. i. rewriter. }
+      { hexploit (@Csharpminor_eval_exprlist_determ bl vargs vargs0); et. i. rewriter.
+        hexploit external_call_determ; [eapply H0|eapply H12|..]. i. des.
+        inv H1. hexploit H2; et. i. des. clarify. }
+      { hexploit (@Csharpminor_eval_expr_determ a v v0); et. i. rewriter.
+        inv H0; inv H12; auto. }
+      { hexploit (@Csharpminor_eval_expr_determ a v v0); et. i. rewriter.
+        inv H0; inv H12; et. }
+      { hexploit (@Csharpminor_eval_expr_determ a v v0); et. i. rewriter. }
+      { hexploit (@alloc_variables_determ (fn_vars f) e e0); et. i. des; clarify. }
+      { hexploit external_call_determ; [eapply H|eapply H6|..]. i. des.
+        inv H0. hexploit H1; et. i. des. clarify. }
+    }
+    { i. inv FINAL. inv STEP. }
+    { i. inv FINAL0. inv FINAL1. ss. }
+  Qed. *)
